Rename strm to ilist

nola/examples/logic/verify/ilist.v
@@ -1,26 +1,26 @@
-(** * Verification on shared mutable singly linked streams *)
+(** * Verification on shared mutable singly linked infinite lists *)
 
-From nola.examples.logic Require Export inv verify.strm_base.
+From nola.examples.logic Require Export inv verify.ilist_base.
 From nola.iris Require Export wp.
 From nola.examples.heap_lang Require Export proofmode notation.
 
-(** Stream whose elements satisfy the condition [Φ] *)
-Definition strm {κ Γᵘ Γᵍ} (N N' : namespace) (Φ : loc → nPropL (;ᵞ Γᵘ ++ Γᵍ))
+(** Infinite list whose elements satisfy the condition [Φ] *)
+Definition ilist {κ Γᵘ Γᵍ} (N N' : namespace) (Φ : loc → nPropL (;ᵞ Γᵘ ++ Γᵍ))
   : loc → nProp κ (Γᵘ;ᵞ Γᵍ) :=
   (rec:ˢ l, n_inv' (_::_) 0 N (¢ᵍ Φ l) ∗
     n_inv' (_::_) 0 N' (∃ l' : loc, (l +ₗ 1) ↦ # l' ∗ %ᵍˢ 0@ l'))%n.
 
-(** Substitution over [strm] *)
-Fact strm_nsubst {κ N N' V Φ Ψ l} :
-  strm (κ:=κ) (Γᵘ:=[V]) N N' Φ l /: Ψ = strm (Γᵘ:=[]) N N' (λ l, Φ l /:ᵍ Ψ) l.
+(** Substitution over [ilist] *)
+Fact ilist_nsubst {κ N N' V Φ Ψ l} :
+  ilist (κ:=κ) (Γᵘ:=[V]) N N' Φ l /: Ψ = ilist (Γᵘ:=[]) N N' (λ l, Φ l /:ᵍ Ψ) l.
 Proof. done. Qed.
 
-(** Interpreted [strm] *)
-Definition strmtl {κ} N N' (Φ : _ → _ (;ᵞ)) l : nProp κ (;ᵞ) :=
-  ∃ l' : loc, (l +ₗ 1) ↦ # l' ∗ strm (Γᵘ:=[]) N N' Φ l'.
-Definition strmi `{!nintpGS Σ} d N N' Φ l : iProp Σ :=
-  nninv d 0 N (Φ l) ∗ nninv d 0 N' (strmtl N N' Φ l).
-Notation strmis := (strmi nderiv).
+(** Interpreted [ilist] *)
+Definition ilisttl {κ} N N' (Φ : _ → _ (;ᵞ)) l : nProp κ (;ᵞ) :=
+  ∃ l' : loc, (l +ₗ 1) ↦ # l' ∗ ilist (Γᵘ:=[]) N N' Φ l'.
+Definition ilisti `{!nintpGS Σ} d N N' Φ l : iProp Σ :=
+  nninv d 0 N (Φ l) ∗ nninv d 0 N' (ilisttl N N' Φ l).
+Notation ilistis := (ilisti nderiv).
 
 (** A has_multiplier of [d] is stored at [l] *)
 Definition has_mult {κ Γ} (d : Z) l : nProp κ Γ := ∃ k, l ↦ #(k * d).
@@ -40,15 +40,15 @@ Definition may_incr_cas (d : Z) : val :=
 Section verify.
   Context `{!nintpGS Σ}.
 
-  (** [strm] is interpreted into [strmi] *)
-  Fact strm_strmi {κ N N' Φ l d} :
-    ⟦ strm N N' Φ l ⟧{κ}(d) ⊣⊢ strmi d N N' Φ l.
+  (** [ilist] is interpreted into [ilisti] *)
+  Fact ilist_ilisti {κ N N' Φ l d} :
+    ⟦ ilist N N' Φ l ⟧{κ}(d) ⊣⊢ ilisti d N N' Φ l.
   Proof. by rewrite/= rew_eq_hwf /=. Qed.
 
-  (** Convert the predicate of [strmi] *)
-  Lemma strmi_convert `{!nderivy Σ ih d} {N N' Φ Ψ l} :
+  (** Convert the predicate of [ilisti] *)
+  Lemma ilisti_convert `{!nderivy Σ ih d} {N N' Φ Ψ l} :
     □ ⸨ ∀ l, (Φ l ={∅}=∗ Ψ l) ∗ (Ψ l ={∅}=∗ Φ l) ⸩(d, 0) -∗
-    strmi d N N' Φ l -∗ strmi d N N' Ψ l.
+    ilisti d N N' Φ l -∗ ilisti d N N' Ψ l.
   Proof.
     move: d nderivy0 Φ Ψ l. apply (derivy_acc (λ _, ∀ Φ Ψ l, _ -∗ _)).
     move=> d ? Φ Ψ l. iIntros "#? #[??]".
@@ -56,55 +56,55 @@ Section verify.
     { iApply derivy_map; [|done]=>/=. iIntros (d' dyd' _) "Φ↔Ψ Φ".
       iDestruct ("Φ↔Ψ" $! _) as "[ΦΨ ΨΦ]". iMod ("ΦΨ" with "Φ") as "$".
       iIntros "!> Ψ". by iApply "ΨΦ". }
-    iApply derivy_byintp=>/=. iIntros (d' dyd' [IH _]) "_ #to _ (%l' & ↦ & s)".
-    iModIntro. rewrite rew_eq_hwf /=. iDestruct "s" as "#s".
+    iApply derivy_byintp=>/=. iIntros (d' dyd' [IH _]) "_ #to _ (%l' & ↦ & i)".
+    iModIntro. rewrite rew_eq_hwf /=. iDestruct "i" as "#i".
     iDestruct ("to" with "[//]") as "?". iSplitL.
     { iExists _. iFrame "↦". rewrite rew_eq_hwf /=. by iApply IH. }
-    iIntros "(%l'' & ↦ & s') !>". iExists _. iFrame "↦".
+    iIntros "(%l'' & ↦ & i') !>". iExists _. iFrame "↦".
     rewrite !rew_eq_hwf /=. iApply IH; [|done]. iModIntro.
     iApply (derivy_map (derivy0:=dyd')); [|done]=>/=.
     iIntros (? _ _) "Φ↔'Ψ %". iApply bi.sep_comm. iApply "Φ↔'Ψ".
   Qed.
 
-  (** [strmi] by cons *)
-  Lemma strmi_cons `{!nderivy Σ ih d} {N N' Φ l l'} :
-    nninv d 0 N (Φ l) -∗ strmi d N N' Φ l' -∗ (l +ₗ 1) ↦ #l' =[nninv_wsat d]=∗
-      strmi d N N' Φ l.
+  (** [ilisti] by cons *)
+  Lemma ilisti_cons `{!nderivy Σ ih d} {N N' Φ l l'} :
+    nninv d 0 N (Φ l) -∗ ilisti d N N' Φ l' -∗ (l +ₗ 1) ↦ #l' =[nninv_wsat d]=∗
+      ilisti d N N' Φ l.
   Proof.
-    iIntros "$ #s ↦".
-    iMod (nninv_alloc (strmtl _ _ _ _) with "[↦]") as "$"; [|done].
+    iIntros "$ #i ↦".
+    iMod (nninv_alloc (ilisttl _ _ _ _) with "[↦]") as "$"; [|done].
     simpl. iExists _. iFrame "↦". by rewrite rew_eq_hwf /=.
   Qed.
 
-  (** [strmi] from a one-node loop *)
-  Lemma strmi_loop_1 `{!nderivy Σ ih d} {N N' Φ l} :
+  (** [ilisti] from a one-node loop *)
+  Lemma ilisti_loop_1 `{!nderivy Σ ih d} {N N' Φ l} :
     nninv d 0 N (Φ l) -∗ (l +ₗ 1) ↦ #l =[nninv_wsat d]=∗
-      strmi d N N' Φ l.
+      ilisti d N N' Φ l.
   Proof.
     iIntros "#Φ ↦". iFrame "Φ".
-    iMod (nninv_alloc_rec (strmtl _ _ _ _) with "[↦]") as "$"; [|done].
+    iMod (nninv_alloc_rec (ilisttl _ _ _ _) with "[↦]") as "$"; [|done].
     iIntros "/= #?". iExists _. rewrite rew_eq_hwf /=. by iFrame "↦ Φ".
   Qed.
 
-  (** [strmi] from a two-node loop *)
-  Lemma strmi_loop_2 `{!nderivy Σ ih d} {N N' Φ l l'} :
+  (** [ilisti] from a two-node loop *)
+  Lemma ilisti_loop_2 `{!nderivy Σ ih d} {N N' Φ l l'} :
     nninv d 0 N (Φ l) -∗ nninv d 0 N (Φ l') -∗
     (l +ₗ 1) ↦ #l' -∗ (l' +ₗ 1) ↦ #l =[nninv_wsat d]=∗
-      strmi d N N' Φ l ∗ strmi d N N' Φ l'.
+      ilisti d N N' Φ l ∗ ilisti d N N' Φ l'.
   Proof.
     iIntros "#Φ #Φ' ↦ ↦'". iFrame "Φ Φ'".
-    iMod (nninv_alloc_rec (strmtl _ _ _ _ ∗ strmtl _ _ _ _) with "[↦ ↦']")
+    iMod (nninv_alloc_rec (ilisttl _ _ _ _ ∗ ilisttl _ _ _ _) with "[↦ ↦']")
       as "inv"; last first.
     { simpl. by iDestruct (nninv_split with "inv") as "[$ $]". }
     iIntros "/= itls". iDestruct (nninv_split with "itls") as "[#? #?]".
     iSplitL "↦"; iExists _; rewrite rew_eq_hwf /=; iFrame; by iSplit.
   Qed.
 
-  (** [siter] terminates under [strmis] *)
+  (** [siter] terminates under [ilistis] *)
   Lemma twp_siter {N N' E Φ l} {f : val} {c : nat} : ↑N' ⊆ E →
     (∀ l : loc,
       [[{ nninvd 0 N (Φ l) }]][nninv_wsatd] f #l @ E [[{ RET #(); True }]]) -∗
-    [[{ strmis N N' Φ l }]][nninv_wsatd]
+    [[{ ilistis N N' Φ l }]][nninv_wsatd]
       siter f #c #l @ E
     [[{ RET #(); True }]].
   Proof.
@@ -112,19 +112,19 @@ Section verify.
     iInduction c as [|c] "IH" forall (l) "ihd itl"; wp_rec; wp_pures;
       [by iApply "Ψ"|].
     wp_apply "f"; [done|]. iIntros "_". wp_pures. wp_bind (! _)%E.
-    iMod (nninvd_acc with "itl") as "/=[(%l' & ↦ & s) cl]"; [done|].
-    rewrite rew_eq_hwf /=. iDestruct "s" as "#[??]". wp_load. iModIntro.
+    iMod (nninvd_acc with "itl") as "/=[(%l' & ↦ & i) cl]"; [done|].
+    rewrite rew_eq_hwf /=. iDestruct "i" as "#[??]". wp_load. iModIntro.
     iMod ("cl" with "[↦]") as "_".
     { iExists _. rewrite rew_eq_hwf /=. iFrame "↦". by iSplit. }
     iModIntro. wp_pures. have ->: (S c - 1)%Z = c by lia.
     by iApply ("IH" with "Ψ").
   Qed.
 
-  (** [siter_nd] terminates under [strmis] *)
+  (** [siter_nd] terminates under [ilistis] *)
   Lemma twp_siter_nd {N N' E Φ l} {f : val} : ↑N' ⊆ E →
     (∀ l : loc,
       [[{ nninvd 0 N (Φ l) }]][nninv_wsatd] f #l @ E [[{ RET #(); True }]]) -∗
-    [[{ strmis N N' Φ l }]][nninv_wsatd]
+    [[{ ilistis N N' Φ l }]][nninv_wsatd]
       siter_nd f #l @ E
     [[{ RET #(); True }]].
   Proof.
@@ -132,11 +132,11 @@ Section verify.
     wp_apply twp_ndnat; [done|]. iIntros (?) "_". by wp_apply twp_siter.
   Qed.
 
-  (** [siter_nd_forks] terminates under [strmis] *)
+  (** [siter_nd_forks] terminates under [ilistis] *)
   Lemma twp_siter_nd_forks {N N' E Φ l} {f : val} {c : nat} :
     (∀ l : loc,
       [[{ nninvd 0 N (Φ l) }]][nninv_wsatd] f #l [[{ RET #(); True }]]) -∗
-    [[{ strmis N N' Φ l }]][nninv_wsatd]
+    [[{ ilistis N N' Φ l }]][nninv_wsatd]
       siter_nd_forks f #c #l @ E
     [[{ RET #(); True }]].
   Proof.
@@ -146,11 +146,11 @@ Section verify.
     have ->: (S c - 1)%Z = c by lia. by iApply "IH".
   Qed.
 
-  (** [siter_nd_forks_nd] terminates under [strmis] *)
+  (** [siter_nd_forks_nd] terminates under [ilistis] *)
   Lemma twp_siter_nd_forks_nd {N N' E Φ l} {f : val} :
     (∀ l : loc,
       [[{ nninvd 0 N (Φ l) }]][nninv_wsatd] f #l [[{ RET #(); True }]]) -∗
-    [[{ strmis N N' Φ l }]][nninv_wsatd]
+    [[{ ilistis N N' Φ l }]][nninv_wsatd]
       siter_nd_forks_nd f #l @ E
     [[{ RET #(); True }]].
   Proof.
