nola/examples/logic/verify/na_ilist.v
@@ -1,40 +1,40 @@
-(** * Verification on non-atomic shared mutable singly linked streams *)
+(** * Verification on non-atomic shared mutable singly linked infinite lists *)
 
-From nola.examples.logic Require Export na_inv verify.strm_base.
+From nola.examples.logic Require Export na_inv verify.ilist_base.
 From nola.iris Require Export wp.
 From nola.examples.heap_lang Require Export proofmode notation.
 
-(** Stream whose elements satisfy the condition [Φ] *)
-Definition na_strm {κ Γᵘ Γᵍ} (p : na_inv_pool_name) (N N' : namespace)
+(** Infinite list whose elements satisfy the condition [Φ] *)
+Definition na_ilist {κ Γᵘ Γᵍ} (p : na_inv_pool_name) (N N' : namespace)
   (Φ : loc → nPropL (;ᵞ Γᵘ ++ Γᵍ)) : loc → nProp κ (Γᵘ;ᵞ Γᵍ) :=
   (rec:ˢ l, n_na_inv' (_::_) 0 p N (¢ᵍ Φ l) ∗
     n_na_inv' (_::_) 0 p N' (∃ l' : loc, (l +ₗ 1) ↦ # l' ∗ %ᵍˢ 0@ l'))%n.
 
-(** Substitution over [na_strm] *)
-Fact na_strm_nsubst {κ p N N' V Φ Ψ l} :
-  na_strm (κ:=κ) (Γᵘ:=[V]) p N N' Φ l /: Ψ =
-    na_strm (Γᵘ:=[]) p N N' (λ l, Φ l /:ᵍ Ψ) l.
+(** Substitution over [na_ilist] *)
+Fact na_ilist_nsubst {κ p N N' V Φ Ψ l} :
+  na_ilist (κ:=κ) (Γᵘ:=[V]) p N N' Φ l /: Ψ =
+    na_ilist (Γᵘ:=[]) p N N' (λ l, Φ l /:ᵍ Ψ) l.
 Proof. done. Qed.
 
-(** Interpreted [strm] *)
-Definition na_strmtl {κ} p N N' (Φ : _ → _ (;ᵞ)) l : nProp κ (;ᵞ) :=
-  ∃ l' : loc, (l +ₗ 1) ↦ # l' ∗ na_strm (Γᵘ:=[]) p N N' Φ l'.
-Definition na_strmi `{!nintpGS Σ} d p N N' Φ l : iProp Σ :=
-  na_nninv d 0 p N (Φ l) ∗ na_nninv d 0 p N' (na_strmtl p N N' Φ l).
-Notation na_strmis := (na_strmi nderiv).
+(** Interpreted [ilist] *)
+Definition na_ilisttl {κ} p N N' (Φ : _ → _ (;ᵞ)) l : nProp κ (;ᵞ) :=
+  ∃ l' : loc, (l +ₗ 1) ↦ # l' ∗ na_ilist (Γᵘ:=[]) p N N' Φ l'.
+Definition na_ilisti `{!nintpGS Σ} d p N N' Φ l : iProp Σ :=
+  na_nninv d 0 p N (Φ l) ∗ na_nninv d 0 p N' (na_ilisttl p N N' Φ l).
+Notation na_ilistis := (na_ilisti nderiv).
 
 Section verify.
   Context `{!nintpGS Σ}.
 
-  (** [na_strm] is interpreted into [na_strmi] *)
-  Fact na_strm_strmi {κ p N N' Φ l d} :
-    ⟦ na_strm p N N' Φ l ⟧{κ}(d) ⊣⊢ na_strmi d p N N' Φ l.
+  (** [na_ilist] is interpreted into [na_ilisti] *)
+  Fact na_ilist_ilisti {κ p N N' Φ l d} :
+    ⟦ na_ilist p N N' Φ l ⟧{κ}(d) ⊣⊢ na_ilisti d p N N' Φ l.
   Proof. by rewrite/= rew_eq_hwf /=. Qed.
 
-  (** Convert the predicate of [na_strmi] *)
-  Lemma na_strmi_convert `{!nderivy Σ ih d} {p N N' Φ Ψ l} :
+  (** Convert the predicate of [na_ilisti] *)
+  Lemma na_ilisti_convert `{!nderivy Σ ih d} {p N N' Φ Ψ l} :
     □ ⸨ ∀ l, (Φ l ={∅}=∗ Ψ l) ∗ (Ψ l ={∅}=∗ Φ l) ⸩(d, 0) -∗
-    na_strmi d p N N' Φ l -∗ na_strmi d p N N' Ψ l.
+    na_ilisti d p N N' Φ l -∗ na_ilisti d p N N' Ψ l.
   Proof.
     move: d nderivy0 Φ Ψ l. apply (derivy_acc (λ _, ∀ Φ Ψ l, _ -∗ _)).
     move=> d ? Φ Ψ l. iIntros "#sΦ↔Ψ #[??]".
@@ -42,53 +42,53 @@ Section verify.
     { iApply derivy_map; [|done]=>/=. iIntros (d' sys' _) "Φ↔Ψ Φ".
       iDestruct ("Φ↔Ψ" $! _) as "[ΦΨ ΨΦ]". iMod ("ΦΨ" with "Φ") as "$".
       iIntros "!> Ψ". by iApply "ΨΦ". }
-    iApply derivy_byintp=>/=. iIntros (d' sys' [IH _]) "_ #to _ (%l' & ↦ & s)".
-    iModIntro. rewrite rew_eq_hwf /=. iDestruct "s" as "#s".
+    iApply derivy_byintp=>/=. iIntros (d' sys' [IH _]) "_ #to _ (%l' & ↦ & i)".
+    iModIntro. rewrite rew_eq_hwf /=. iDestruct "i" as "#i".
     iDestruct ("to" with "[//]") as "?". iSplitL.
     { iExists _. iFrame "↦". rewrite rew_eq_hwf /=. by iApply IH. }
-    iIntros "(%l'' & ↦ & s') !>". iExists _. iFrame "↦".
+    iIntros "(%l'' & ↦ & i') !>". iExists _. iFrame "↦".
     rewrite !rew_eq_hwf /=. iApply IH; [|done]. iModIntro.
     iApply (derivy_map (derivy0:=sys')); [|done]=>/=.
     iIntros (? _ _) "Φ↔'Ψ %". iApply bi.sep_comm. iApply "Φ↔'Ψ".
   Qed.
 
-  (** [na_strmi] by cons *)
-  Lemma na_strmi_cons `{!nderivy Σ ih d} {p N N' Φ l l'} :
-    na_nninv d 0 p N (Φ l) -∗ na_strmi d p N N' Φ l' -∗ (l +ₗ 1) ↦ #l'
-      =[nninv_wsat d]=∗ na_strmi d p N N' Φ l.
+  (** [na_ilisti] by cons *)
+  Lemma na_ilisti_cons `{!nderivy Σ ih d} {p N N' Φ l l'} :
+    na_nninv d 0 p N (Φ l) -∗ na_ilisti d p N N' Φ l' -∗ (l +ₗ 1) ↦ #l'
+      =[nninv_wsat d]=∗ na_ilisti d p N N' Φ l.
   Proof.
-    iIntros "$ #s ↦".
-    iMod (na_nninv_alloc (na_strmtl _ _ _ _ _) with "[↦]") as "$"; [|done].
+    iIntros "$ #i ↦".
+    iMod (na_nninv_alloc (na_ilisttl _ _ _ _ _) with "[↦]") as "$"; [|done].
     simpl. iExists _. iFrame "↦". by rewrite rew_eq_hwf /=.
   Qed.
 
-  (** [na_strmi] from a one-node loop *)
-  Lemma na_strmi_loop_1 `{!nderivy Σ ih d} {p N N' Φ l} :
+  (** [na_ilisti] from a one-node loop *)
+  Lemma na_ilisti_loop_1 `{!nderivy Σ ih d} {p N N' Φ l} :
     na_nninv d 0 p N (Φ l) -∗ (l +ₗ 1) ↦ #l =[nninv_wsat d]=∗
-      na_strmi d p N N' Φ l.
+      na_ilisti d p N N' Φ l.
   Proof.
     iIntros "#Φ ↦". iFrame "Φ".
-    iMod (na_nninv_alloc_rec (na_strmtl _ _ _ _ _) with "[↦]") as "$"; [|done].
+    iMod (na_nninv_alloc_rec (na_ilisttl _ _ _ _ _) with "[↦]") as "$"; [|done].
     iIntros "/= #?". iExists _. rewrite rew_eq_hwf /=. by iFrame "↦ Φ".
   Qed.
 
-  (** [na_strmi] from a two-node loop *)
-  Lemma na_strmi_loop_2 `{!nderivy Σ ih d} {p N N' Φ l l'} :
+  (** [na_ilisti] from a two-node loop *)
+  Lemma na_ilisti_loop_2 `{!nderivy Σ ih d} {p N N' Φ l l'} :
     na_nninv d 0 p N (Φ l) -∗ na_nninv d 0 p N (Φ l') -∗
     (l +ₗ 1) ↦ #l' -∗ (l' +ₗ 1) ↦ #l =[nninv_wsat d]=∗
-      na_strmi d p N N' Φ l ∗ na_strmi d p N N' Φ l'.
+      na_ilisti d p N N' Φ l ∗ na_ilisti d p N N' Φ l'.
   Proof.
     iIntros "#Φ #Φ' ↦ ↦'". iFrame "Φ Φ'".
-    iMod (na_nninv_alloc_rec (na_strmtl _ _ _ _ _ ∗ na_strmtl _ _ _ _ _)
+    iMod (na_nninv_alloc_rec (na_ilisttl _ _ _ _ _ ∗ na_ilisttl _ _ _ _ _)
       with "[↦ ↦']") as "inv"; last first.
     { simpl. by iDestruct (na_nninv_split with "inv") as "[$ $]". }
     iIntros "/= itls". iDestruct (na_nninv_split with "itls") as "[#? #?]".
     iSplitL "↦"; iExists _; rewrite rew_eq_hwf /=; iFrame; by iSplit.
   Qed.
 
-  (** [siter] terminates under [na_strmis] *)
+  (** [siter] terminates under [na_ilistis] *)
   Lemma twp_siter_na {p N N' Φ E F l} {f : val} {c : nat} : ↑N' ⊆ E → ↑N' ⊆ F →
-    na_strmis p N N' Φ l -∗
+    na_ilistis p N N' Φ l -∗
     (∀ l, [[{ na_nninvd 0 p N (Φ l) ∗ na_own p F }]][nninv_wsatd]
             f #l @ E
           [[{ RET #(); na_own p F }]]) -∗
@@ -100,17 +100,17 @@ Section verify.
     iInduction c as [|c] "IH" forall (l) "ihd itl"; wp_rec; wp_pures;
       [by iApply "Ψ"|].
     wp_apply ("f" with "[$pF //]"). iIntros "pF". wp_pures. wp_bind (! _)%E.
-    iMod (na_nninvd_acc with "[//] pF") as "/=((%l' & ↦ & s) & pF∖N & cl)";
+    iMod (na_nninvd_acc with "[//] pF") as "/=((%l' & ↦ & i) & pF∖N & cl)";
       [done..|].
-    rewrite rew_eq_hwf /=. iDestruct "s" as "#[??]". wp_load. wp_pures.
+    rewrite rew_eq_hwf /=. iDestruct "i" as "#[??]". wp_load. wp_pures.
     iMod ("cl" with "[↦] pF∖N") as "pF".
     { iExists _. iFrame "↦". rewrite/= rew_eq_hwf /=. by iSplit. }
     have ->: (S c - 1)%Z = c by lia. by iApply ("IH" with "pF Ψ").
   Qed.
 
-  (** [siter_nd] terminates under [na_strmis] *)
+  (** [siter_nd] terminates under [na_ilistis] *)
   Lemma twp_siter_nd_na {p N N' Φ E F l} {f : val} : ↑N' ⊆ E → ↑N' ⊆ F →
-    na_strmis p N N' Φ l -∗
+    na_ilistis p N N' Φ l -∗
     (∀ l, [[{ na_nninvd 0 p N (Φ l) ∗ na_own p F }]][nninv_wsatd]
             f #l @ E
           [[{ RET #(); na_own p F }]]) -∗
